adding basic lemmas for bits insert and bits extract

theory/rBPFCommType.thy
@@ -54,7 +54,7 @@ abbreviation bit_right_shift ::
   "'a :: len word \<Rightarrow> nat \<Rightarrow> 'a :: len word" (infix ">>" 50)
   where "x >> n \<equiv> drop_bit n x"
 
-fun unsigned_bitfield_extract_u8 :: "nat \<Rightarrow> nat \<Rightarrow> u8 \<Rightarrow> u8" where
+definition unsigned_bitfield_extract_u8 :: "nat \<Rightarrow> nat \<Rightarrow> u8 \<Rightarrow> u8" where
 "unsigned_bitfield_extract_u8 pos width n = and ((2 ^ width) - 1) (n >> pos)"
 
 definition bitfield_insert_u8 :: "nat \<Rightarrow> nat \<Rightarrow> u8 \<Rightarrow> u8 \<Rightarrow> u8" where
@@ -122,5 +122,267 @@ definition u8_list_of_u64 :: "u64 \<Rightarrow> u8 list" where
 lemma [simp]: "u8_of_bool False = 0" by (unfold u8_of_bool_def, simp)
 
 lemma [simp]: "u8_of_bool True = 1" by (unfold u8_of_bool_def, simp)
+
+lemma add_commute_nat: "a + b = b + (a::nat)" by simp
+
+lemma add_commute_u8: "a + b = b + (a::u8)" by simp
+
+lemma and_truel: "(a \<and> b = b) = (a = True)" by simp
+
+lemma bits_zero_ext_u8 [simp]: "\<And>n x i. 0 \<le> i \<Longrightarrow>
+  bit (and ((2 ^ n) - 1) (x::u8)) i = (if i < n then bit x i else False)"
+  apply (induct_tac n, simp_all add: bit_simps)
+  by (smt (verit) bit_1_0 bit_iff_odd bit_imp_le_length
+      cancel_comm_monoid_add_class.diff_cancel even_mask_div_iff
+      even_mult_exp_div_word_iff less_antisym mult.right_neutral
+      not_less one_add_one power.simps(2) square_diff_one_factored)
+
+lemma bits_shl_u8 [simp]: "\<And>(x::u8) y i. 0 \<le> i \<Longrightarrow> i < 8 \<Longrightarrow>
+  bit (x << y) i = (if i < y then False else bit x (i - y))"
+  subgoal for x y i by (cases "i < y", simp_all add: bit_simps)
+  done
+
+lemma bits_mod_two_p_u8 [simp]: "0 \<le> n \<Longrightarrow> 0 \<le> i \<Longrightarrow>
+  bit ((x::u8) mod (2 ^ n)) i = (if i < n then bit x i else False)"
+  apply (induction n arbitrary: x i, simp_all add: bit_simps)
+  subgoal for n x i
+    apply (cases "i < n", simp_all add: bit_simps)
+    subgoal by (metis bit_take_bit_iff less_Suc_eq power_Suc take_bit_eq_mod)
+    subgoal
+      by (metis bit_take_bit_iff power_Suc take_bit_eq_mod) 
+    done
+  done
+
+lemma [simp]:"\<And>(a::u8) b c. a + (b + c) = (a + c) + b"
+  by simp
+
+(*
+lemma mod_unique_u8: "\<And>(a::u8) b q r. 0 \<le> a \<Longrightarrow> 0 \<le> r \<Longrightarrow> r < b \<Longrightarrow>
+  a = b*q+r \<Longrightarrow> r = a mod b"
+  subgoal for a b q r
+ *)
+
+(**r
+mod_unique:
+ forall a b q r, 0<=a -> 0<=r<b ->
+  a == b*q + r -> r == a mod b.
+Proof.
+intros a b q r Ha (Hb,Hr) EQ.
+destruct (div_mod_unique b q (a/b) r (a mod b)); auto.
+- apply mod_bound_pos; order.
+- rewrite <- div_mod; order.
+Qed.
+
+*)
+
+(*
+lemma mod_add_u8: "\<And>(a::u8) b c. 0 \<le> a \<Longrightarrow> 0 \<le> a+b*c \<Longrightarrow> 0 < c \<Longrightarrow>
+  (a + b * c) mod c == a mod c"
+  subgoal for a b c
+*)
+
+(**r
+
+Lemma mod_add : forall a b c, 0<=a -> 0<=a+b*c -> 0<c ->
+ (a + b * c) mod c == a mod c.
+Proof.
+ intros a b c ? ? ?.
+ symmetry.
+ apply mod_unique with (a/c+b); auto.
+ - apply mod_bound_pos; auto.
+ - rewrite mul_add_distr_l, add_shuffle0, <- div_mod by order.
+   now rewrite mul_comm.
+Qed.
+
+*)
+
+(*
+lemma mod_plus_u8: "\<And>(a::u8) b c. (a + b * c) mod c = a mod c"
+  subgoal for a b c
+    apply (cases "c = 0", simp_all)
+*)
+
+(**r 
+
+Lemma Z_mod_plus_full : forall a b c:Z, (a + b * c) mod c = a mod c.
+Proof. intros a b c. zero_or_not c.
+ - now rewrite Z.mul_0_r, Z.add_0_r.
+ - now apply Z.mod_add.
+Qed.
+
+*)
+
+
+(*
+lemma mod_unique_u8: "\<And>(x::u8) y a b. x = a * y + b \<Longrightarrow> 0 \<le> b \<Longrightarrow> b < y \<Longrightarrow> x mod y = b"
+  subgoal for x y a b
+    apply (simp add: add_commute_u8)
+*)
+
+(**r 
+(a + b * c) mod c = a mod c
+Lemma Zmod_unique:
+  forall x y a b,
+  x = a * y + b -> 0 <= b < y -> x mod y = b.
+Proof.
+  intros. subst x. rewrite Z.add_comm.
+  rewrite Z_mod_plus. apply Z.mod_small. auto. lia.
+Qed.
+
+*)
+
+(*
+lemma [simp]: "\<And>(n::nat). ((two_p n - 1)::u8) = (((-1)::u8) mod (two_p n))"
+  subgoal for n
+
+lemma bits_two_p_m1_u8: "\<And>n i. bit ((2 ^ n - 1)::u8) i = (if i < n then True else False)"
+
+  apply (induct_tac n, simp_all add: bit_simps)
+  subgoal for i n
+    apply (simp add: bits_mod_two_p_u8)
+    subgoal 
+
+      done
+*)
+
+(**r
+Ztestbit_two_p_m1:
+  forall n i, 0 <= n -> 0 <= i ->
+  Z.testbit (two_p n - 1) i = if zlt i n then true else false.
+Proof.
+  intros. replace (two_p n - 1) with ((-1) mod (two_p n)).
+  rewrite Ztestbit_mod_two_p; auto. destruct (zlt i n); auto. apply Ztestbit_m1; auto.
+  apply Zmod_unique with (-1). ring.
+  exploit (two_p_gt_ZERO n). auto. lia.
+Qed.
+
+*)
+
+lemma bits_unsigned_bitfield_extract_u8: "\<And>pos width n i.
+  0 \<le> pos \<Longrightarrow> 0 < width \<Longrightarrow> pos + width \<le> 8 \<Longrightarrow>
+  0 \<le> i \<Longrightarrow> i < 8 \<Longrightarrow> \<comment> \<open> TODO: i \<le> 8 is also OK !!  \<close>
+  bit (unsigned_bitfield_extract_u8 pos width n) i =
+  (if i < width then bit n (i + pos) else False)"
+  subgoal for pos width n i
+    apply (unfold unsigned_bitfield_extract_u8_def)
+    apply (simp only: bits_zero_ext_u8)
+    apply (cases "i < width", simp_all add: bit_simps)
+    apply (simp add: add_commute_nat)
+        \<comment> \<open> TODO: why Isabell/HOL can not do Nat.add_commute automatically \<close>
+    done
+  done
+
+lemma [simp]: "\<not> (i::nat) < pos \<Longrightarrow> (i - pos < width) = (i < pos + width)"
+  by (simp add: add_commute_nat less_diff_conv2)
+
+lemma bits_bitfield_insert_u8: "\<And>pos width n p i.
+  0 \<le> pos \<Longrightarrow> 0 < width \<Longrightarrow> pos + width \<le> 8 \<Longrightarrow>
+  0 \<le> i \<Longrightarrow> i < 8 \<Longrightarrow>
+  bit (bitfield_insert_u8 pos width n p) i =
+  (if pos \<le> i \<and> i < (pos + width) then bit p (i - pos) else bit n i)"
+  subgoal for pos width n p i
+    apply (unfold bitfield_insert_u8_def Let_def)
+    apply (simp only: bit_or_iff)
+    apply (simp only: bit_and_iff)
+    apply (simp only: bit_not_iff)
+    apply (simp only: bits_shl_u8)
+    apply (simp only: bits_zero_ext_u8)
+    apply (cases "i < pos", simp_all)
+\<comment> \<open> TODO: We try a stupid way now \<close>
+    apply (cases i, simp_all add: bit_1_iff bit_0)
+    subgoal for i1 apply (cases i1, simp_all)
+       apply (smt (verit) One_nat_def Suc_diff_eq_diff_pred add_diff_cancel_left' bit_and_iff
+          bits_zero_ext_u8 diff_diff_cancel le0 leI not_gr_zero odd_bit_iff_bit_pred plus_1_eq_Suc
+          semiring_parity_class.even_mask_iff zero_less_diff)
+
+      subgoal for i2 apply (cases i2, simp_all)
+        subgoal apply (cases pos, simp_all)
+          apply (meson bit_and_iff bits_zero_ext_u8 le0)
+          subgoal for pos1
+            by (smt (verit, del_insts) Suc_le_eq Suc_lessI add_diff_cancel_left' bit_iff_odd
+                bit_imp_le_length diff_is_0_eq' diff_zero even_mask_div_iff leI less_le_not_le) 
+          done
+
+        subgoal for i3 apply (cases i3, simp_all)
+          subgoal apply (cases pos, simp_all)
+            apply (meson bit_iff_odd even_mask_div_iff exp_eq_0_imp_not_bit linorder_not_less)
+            subgoal for pos1
+              by (smt (verit) Suc_le_eq add_diff_cancel_left' bit_iff_odd bit_imp_le_length
+                  diff_is_0_eq' diff_zero even_mask_div_iff exp_eq_zero_iff leI less_Suc_eq
+                  less_le_not_le plus_1_eq_Suc zero_less_Suc)
+            done
+
+          subgoal for i4 apply (cases i4, simp_all)
+            subgoal apply (cases pos, simp_all)
+              apply (meson bit_iff_odd even_mask_div_iff exp_eq_0_imp_not_bit linorder_not_less)
+              subgoal for pos1
+                by (smt (verit) One_nat_def Suc_diff_eq_diff_pred Suc_pred add_diff_cancel_left' 
+                    bit_iff_odd bot_nat_0.not_eq_extremum cancel_comm_monoid_add_class.diff_cancel
+                    diff_is_0_eq' even_mask_div_iff exp_eq_0_imp_not_bit le_Suc_eq less_SucE
+                    less_diff_conv mult.right_neutral not_less_eq one_add_one plus_1_eq_Suc
+                    power.simps(2) square_diff_one_factored)
+              done
+
+            subgoal for i5 apply (cases i5, simp_all)
+              subgoal apply (cases pos, simp_all)
+                apply (meson bit_iff_odd even_mask_div_iff exp_eq_0_imp_not_bit linorder_not_less)
+                subgoal for pos1
+                  by (smt (verit) One_nat_def Suc_diff_eq_diff_pred Suc_pred add_diff_cancel_left' 
+                      bit_iff_odd bot_nat_0.not_eq_extremum cancel_comm_monoid_add_class.diff_cancel
+                      diff_is_0_eq' even_mask_div_iff exp_eq_0_imp_not_bit le_Suc_eq less_SucE
+                      less_diff_conv mult.right_neutral not_less_eq one_add_one plus_1_eq_Suc
+                      power.simps(2) square_diff_one_factored)
+                done
+
+              subgoal for i6 apply (cases i6, simp_all)
+                subgoal apply (cases pos, simp_all)
+                   apply (meson bit_iff_odd even_mask_div_iff exp_eq_0_imp_not_bit linorder_not_less)
+                  subgoal for pos1
+                    by (smt (verit) One_nat_def Suc_diff_eq_diff_pred Suc_pred add_diff_cancel_left' 
+                        bit_iff_odd bot_nat_0.not_eq_extremum cancel_comm_monoid_add_class.diff_cancel
+                        diff_is_0_eq' even_mask_div_iff exp_eq_0_imp_not_bit le_Suc_eq less_SucE
+                        less_diff_conv mult.right_neutral not_less_eq one_add_one plus_1_eq_Suc
+                        power.simps(2) square_diff_one_factored)
+                  done
+
+                subgoal for i7 apply (cases i7, simp_all)
+                  subgoal apply (cases pos, simp_all)
+                     apply (meson bit_iff_odd even_mask_div_iff exp_eq_0_imp_not_bit linorder_not_less)
+                    subgoal for pos1
+                      by (smt (verit) One_nat_def Suc_diff_eq_diff_pred Suc_pred add_diff_cancel_left' 
+                          bit_iff_odd bot_nat_0.not_eq_extremum cancel_comm_monoid_add_class.diff_cancel
+                          diff_is_0_eq' even_mask_div_iff exp_eq_0_imp_not_bit le_Suc_eq less_SucE
+                          less_diff_conv mult.right_neutral not_less_eq one_add_one plus_1_eq_Suc
+                          power.simps(2) square_diff_one_factored)
+                    done
+                  done
+                done
+              done
+            done
+          done
+        done
+      done
+    done
+  done
+
+
+(*
+    apply (cases "i - pos < width", simp_all)
+    subgoal 
+
+*)
+
+
+(**r
+
+  destruct (zlt i pos).
+- unfold proj_sumbool; rewrite zle_false by lia. cbn. apply andb_true_r.
+- unfold proj_sumbool; rewrite zle_true by lia; cbn.
+  rewrite bits_zero_ext, testbit_repr, Ztestbit_two_p_m1 by lia.
+  destruct (zlt (i - pos) width); cbn.
++ rewrite zlt_true by lia. rewrite andb_false_r, orb_false_r. auto.
++ rewrite zlt_false by lia. apply andb_true_r.
+
+*)
 
 end
